---
layout: post
title: "Robustness of Tukey Median"
---
The Tukey median  introduced in
[the previous post]({{ site.baseurl }}{% post_url 2022-12-16-introduction-of-tukey-median %})
robustly estimates the true mean, i.e., the mean of the distribution 
before contaminated by outliers, or sample corruption.
Specifically, 
letting $S \subset \mathbb{R}^{d}$ be an $\epsilon$-corrupted set of samples of size $n$ from $\mathcal{N}(\mu, \text{I}\_{d})$,
where $\epsilon \lt \frac{1}{6}$,
there exists some universal constant $C \lt 0$ so that with probability $1 âˆ’ \delta$, and we have that
\\[
    \lVert \text{Tukey}(S) - \mu \rVert_{2} \leq \Phi^{-1}
    \left (
    \frac{1}{2} + 3 \epsilon + 
    C \sqrt{ \frac{d + \log 1/\delta}{n} }
    \right ).
    \label{eq:1}\tag{1}
\\]
We saw that In particular, when $n$ is sufficiently large and $\epsilon$ is relatively small,
the error in the mean estimation becomes
\\[
    \lVert \text{Tukey}(S) - \mu \rVert_{2} 
    \simeq \Phi^{-1}
    \left (
    \frac{1}{2} + 3 \epsilon + 
    \right )
    = O(\epsilon).
    \label{eq:2}\tag{2}
\\]
We will proof Eq.$\,$($\ref{eq:1}$). 

## $d$-dimension to 1-dimension with Gaussian CDF
Assuming $\forall \lVert v \rVert_{2} = 1$, we suppose
\\[
    \frac{ |\\{ x \in S_{g}: \langle x - \eta, v \rangle \geq 0\\}|} {|S_{g}|}
    =
    \color{blue}{
    \mathbb{P}\_{x \sim \mathcal{N}(\mu, \text{I}\_{d})} \left \lbrack \langle x - \eta, v \rangle \geq 0 \right \rbrack,
    }
    \label{eq:3}\tag{3}
\\]
sayings that let's ignore the concentraion of $\mathcal{N}(\mu, \text{I}\_{d})$ for now.
We first show that 
\\[
    \color{blue}{
    \mathbb{P}\_{x \sim \mathcal{N}(\mu, \text{I}\_{d})} \left \lbrack \langle x - \eta, v \rangle \geq 0 \right \rbrack
    }
    =
    \color{green}{
    \Phi(\langle \mu - \eta, v \rangle)
    }.
\\]
As $\langle x - \eta, v \rangle \geq 0 $ can be written as 
\\[
    \langle x,  v \rangle \geq \langle \eta,  v \rangle
    \Leftrightarrow
    \langle x - \mu,  v \rangle \geq \langle \eta - \mu,  v \rangle,
\\]
defining $z$ as $z := x - \mu$, we have $\langle z, v \rangle \geq  \langle \eta - \mu, v \rangle$.
Transformation from $x$ to $z$ is shown below:

![z = x - mu]({{site.baseurl}}/img/Tukey/fig_eta_mu.png){: .centered width="800" }

Thus, we have
\\[
    \color{blue}{
    \mathbb{P}\_{x \sim \mathcal{N}(\mu, \text{I}\_{d})} \left \lbrack \langle x - \eta, v \rangle \geq 0 \right \rbrack
    }
    =
    \mathbb{P}\_{z \sim \mathcal{N}(0, \text{I}\_{d})} 
    \left \lbrack 
    \langle z, v \rangle 
    \geq
    \langle \mu - \eta, v \rangle
    \right \rbrack.
\\]

The $z$ satisfying $\langle z, v \rangle \geq \langle \eta - \mu, v \rangle$ corresponds to the points in the yellow region in the figure below.

![\<z,v\>]({{site.baseurl}}/img/Tukey/fig_z_v.png){: .centered width="400" }

Then, as shown below,

![Gaussian CDF]({{site.baseurl}}/img/Tukey/fig_eta_mu_to_phi.png){: .centered width="300" }

we know 
\\[
    \mathbb{P}\_{z \sim \mathcal{N}(0, \text{I}\_{d})} 
    \left \lbrack 
    \langle z, v \rangle 
    \geq
    \langle \mu - \eta, v \rangle
    \right \rbrack
    =
    \color{green}{
    \Phi(\langle \mu - \eta, v \rangle)
    },
\\]
and the proof of Eq.$\,$($\ref{eq:3}$) is done. 

## Rbustness of $\text{Tukey}(S)$
To derive Eqs.$\,$($\ref{eq:1}$) and $\,$($\ref{eq:2}$),
we obtain two claims by using Eqs.$\,$($\ref{eq:3}$).

#### Claim 1
The first claim states that 
\\[
    \text{depth}(S, \mu) \geq \frac{1}{2} n - \epsilon n.
\\]

As $S = S_{g} \setminus S_{r} \cup S_{b}$, for all $\lVert v \rVert_{2} = 1$, we have
\\[
    |\\{ x \in S: \langle x - \mu, v \rangle \geq 0\\}|
    =
    \color {red}{
    |\\{ x \in S_{g}: \langle x - \mu, v \rangle \geq 0\\}|
    }
    +
    |\\{ x \in S_{b}: \langle x - \mu, v \rangle \geq 0\\}|
    -
    |\\{ x \in S_{r}: \langle x - \mu, v \rangle \geq 0\\}|
    .
\\]
What we want now is the lower bound of the above, so we ignore the second term and take the maximamu of the third term utilizing
the assumption of 
$
    |\\{ x \in S_{r}: \langle x - \mu, v \rangle \geq 0\\}| \leq \epsilon n.
$
Then, the above is bounded as
\\[
    \geq 
    \color {red}{
    |\\{ x \in S_{g}: \langle x - \mu, v \rangle \geq 0\\}|
    }
    + 0 - \epsilon n.
\\]

From Eq.$\,$($\ref{eq:3}$), the first term can be written as
\\[
    \color {red}{
    |\\{ x \in S_{g}: \langle x - \mu, v \rangle \geq 0\\}|
    }
    =
    n \mathbb{P}\_{x \sim \mathcal{N}(\mu, \text{I}\_{d})} \left \lbrack \langle x - \mu, v \rangle \geq 0 \right \rbrack
    =
    n \Phi ( \langle \mu - \mu, v \rangle )
    =
    n \Phi ( 0 ) = \frac{1}{2} n,
\\]
and putting them together, we have
\\[
    |\\{ x \in S_{g}: \langle x - \mu, v \rangle \geq 0\\}|
    \geq
    \frac{1}{2} n - \epsilon n.
\\]
It is equivalent to the claim. 

#### Claim 2 
Suppose $\eta \in \mathbb{R}^{d}$ satisifies 
$\lVert \eta - \mu \rVert_{2} \leq \Phi^{-1}(\frac{1}{2} + 3 \epsilon) $.
Then, $\text{depth}(S, \eta) \lt \frac{1}{2} - \epsilon$.

We will derive the upper bound and thus take inequality the other way around from Claim 1.
\\[
    |\\{ x \in S: \langle \eta - \mu, v \rangle \geq 0\\}|
    =
    \color {red}{
    |\\{ x \in S_{g}: \langle \eta - \mu, v \rangle \geq 0\\}|
    }
    +
    |\\{ x \in S_{b}: \langle \eta - \mu, v \rangle \geq 0\\}|
    -
    |\\{ x \in S_{r}: \langle \eta - \mu, v \rangle \geq 0\\}|
\\]
can be bounded as 
\\[
    \leq 
    \color {red}{
    |\\{ x \in S_{g}: \langle \eta - \mu, v \rangle \geq 0\\}|
    }
    + \epsilon n - 0
    \leq 
    n \Phi ( \langle \eta - \mu, v \rangle ) + \epsilon n.
\\]
Selecting $v$ as $v = \frac{\mu - \eta}{\lVert \mu - \eta \rVert_{2} }$, the above becomes
\\[
    = n \Phi ( - \lVert \mu - \eta \rVert_{2}) + \epsilon n.
\\]
Applying the assumption $\lVert \eta - \mu \rVert_{2} \leq \Phi^{-1}(\frac{1}{2} + 3 \epsilon) $,
it is bounded as
\\[
    \leq n (\frac{1}{2} - 3 \epsilon) + \epsilon n = \frac{1}{2} n - 2\epsilon n
    \leq \frac{1}{2} n - \epsilon n,
\\]
and thus it says
\\[
    \text{depth}(S, \eta) \lt \frac{1}{2} - \epsilon .  
\\]

#### Derive Eq.$\,$($\ref{eq:2}$)
Recall $\text{Tukey}(S) = \underset{\eta}{\operatorname{argmax}} \text{depth}(S, \eta)$,
it must be
\\[
    \text{Tukey}(S) \geq \text{depth}(S, \mu) \geq \frac{1}{2} - \epsilon . 
\\]
On the other hand, Claim 2 says that if $\text{depth}(S, \eta) \geq \frac{1}{2} - \epsilon$,
then 
$\lVert \eta - \mu \rVert_{2} \leq \Phi^{-1}(\frac{1}{2} + 3 \epsilon) $.
Thus we obtain
\\[
    \lVert \text{Tukey}(S) - \mu \rVert_{2} 
    \leq
    \Phi^{-1}
    \left (
    \frac{1}{2} + 3 \epsilon
    \right )
    .
\\]
We need to take a few step to achieve Eq.$\,$($\ref{eq:1}$), but we refer the reader to 
[the course note](https://jerryzli.github.io/robust-ml-fall19/lec3.pdf) of Jerry Li.
